\documentclass{article}
\usepackage{amsmath}

\begin{document}

Constraints:

\begin{equation}
X+Y+Z = 1
\end{equation}

\begin{equation}
  Y = Y_{BBN} + \frac{\Delta Y}{\Delta Z} Z
\end{equation}

\begin{equation}
\frac{Z}{X} = \left(\frac{Z}{X}\right)_{\odot} 10^{[Fe/H]}
\end{equation}

Where $Y_{BBN}$, $\left(\frac{Z}{X}\right)_{\odot}$, $\frac{\Delta Y}{\Delta Z}$, and [Fe/H] are given as input.


Even though we don't know X or Z, we know (Z/X) from (3) and the input [Fe/H]. So we treat (Z/X) as a single variable below.

Begin with (1) and isolate Y.

\begin{equation}
  X+Z=1-Y
\end{equation}

Replace Y with (2).

\begin{equation}
  X +Z = 1 - (Y_{BBN} + \frac{\Delta Y}{\Delta Z} Z)
\end{equation}

Replace Z with (Z/X)$\times$X.

 \begin{equation}
 X ( 1 + \frac{Z}{X}) = 1 - (Y_{BBN} + \frac{\Delta Y}{\Delta Z} \frac{Z}{X} X)
\end{equation}

Gather terms with X on the LHS.

\begin{equation}
 X ( 1 + \frac{Z}{X} ( 1 + \frac{\Delta Y}{\Delta Z})) = 1 - Y_{BBN}
\end{equation}

Finally make X all alone on the RHS.

\begin{align}
  X = \frac{1-Y_{BBN}}{ 1 + \frac{Z}{X} ( 1 + \frac{\Delta Y}{\Delta Z})} \\
  Z= \frac{Z}{X} \times X\\
  Y= 1 - X - Z
\end{align}

Done!

\end{document}
